Validator/Regex/Regex.lean
@@ -5,9 +5,8 @@ import Validator.Regex.Lang
 
 -- A regular expression is defined over a generic symbol
 inductive Regex (σ: Type) where
-  | emptyset | emptystr | symbol (s: σ)
-  | or (r1 r2: Regex σ) | concat (r1 r2: Regex σ)
-  | star (r1: Regex σ) | interleave (r1 r2: Regex σ)
+  | emptyset | emptystr | symbol (s: σ) | or (r1 r2: Regex σ)
+  | concat (r1 r2: Regex σ) | star (r1: Regex σ) | interleave (r1 r2: Regex σ)
   | and (r1 r2: Regex σ) | compliment (r1: Regex σ)
   deriving DecidableEq, Ord, Repr, Hashable
 
